src/Bedrock/Field/Synthesis/Examples/X1305_32.v
@@ -1,34 +1,34 @@
 Require Import Coq.ZArith.ZArith.
 Require Import Coq.Lists.List.
 Require Import Coq.Strings.String.
-Require Import Crypto.Bedrock.Field.Translation.Parameters.SelectParameters.
+Require Import Crypto.Bedrock.Field.Translation.Parameters.Defaults32.
 Require Import Crypto.Bedrock.Field.Synthesis.Generic.UnsaturatedSolinas.
 Require Import Crypto.Bedrock.Field.Synthesis.Specialized.UnsaturatedSolinas.
 Local Open Scope Z_scope.
 Import ListNotations.
 
+Local Existing Instances default_parameters default_parameters_ok.
 Local Definition n := 5%nat.
 Local Definition s := 2^130.
 Local Definition c := [(1, 5)].
-Local Definition machine_wordsize := 32.
 Local Definition prefix := "poly1305_"%string.
 
 Instance names : names_of_operations.
   make_names_of_operations prefix. Defined.
 
-Definition ops : unsaturated_solinas_reified_ops n s c machine_wordsize.
+Definition ops : unsaturated_solinas_reified_ops n s c.
 Proof. make_reified_ops. Time Defined.
 
 Instance poly1305_bedrock2_funcs : bedrock2_unsaturated_solinas_funcs.
-funcs_from_ops ops. Defined.
+Proof. funcs_from_ops ops. Defined.
 
 Instance poly1305_bedrock2_specs : bedrock2_unsaturated_solinas_specs.
-specs_from_ops ops n s c. Defined.
+Proof. specs_from_ops ops n s c. Defined.
 
 Instance poly1305_bedrock2_correctness :
   bedrock2_unsaturated_solinas_correctness.
-prove_correctness ops n s c machine_wordsize. Defined.
+Proof. prove_correctness ops n s c. Qed.
 (*
-Eval cbv [add poly1305_bedrock2] in add.
-Eval cbv [spec_of_add poly1305_bedrock2] in spec_of_add.
+Eval cbv [add poly1305_bedrock2_funcs] in add.
+Eval cbv [spec_of_add poly1305_bedrock2_specs] in spec_of_add.
 *)
