src/Bedrock/Field/Translation/Proofs/Flatten.v
@@ -29,18 +29,19 @@ Import Types.Notations.
    conversions between the two. *)
 
 Section Flatten.
-  Context {p : parameters} {p_ok : @ok p}.
+  Context 
+    {width BW word mem locals env ext_spec varname_gen error}
+   `{parameters_sentinel : @parameters width BW word mem locals env ext_spec varname_gen error}.
+  Context {ok : ok}.
   (* these conversions should happen before loading arguments and after
        storing return values, so they use in-memory lists *)
   Local Existing Instance rep.listZ_mem.
   Local Existing Instance rep.Z.
-  Local Instance sem_ok : Semantics.parameters_ok semantics
-    := semantics_ok.
 
   Lemma flatten_base_samelength {t}
         (names : base_ltype t)
         (value : base.interp t) :
-    forall (words : list Semantics.word) s R mem,
+    forall (words : list word) s R mem,
       sep (equivalent_flat_base value words s) R mem ->
       length words = length (flatten_base_ltype names).
   Proof.
@@ -62,7 +63,7 @@ Section Flatten.
   Lemma flatten_args_samelength {t}
         (argnames : type.for_each_lhs_of_arrow ltype t)
         (args : type.for_each_lhs_of_arrow API.interp_type t) :
-    forall (flat_args : list Semantics.word) s mem,
+    forall (flat_args : list word) s mem,
       equivalent_flat_args args flat_args s mem ->
       length flat_args = length (flatten_argnames argnames).
   Proof.
@@ -85,7 +86,7 @@ Section Flatten.
   Lemma of_list_zip_flatten_argnames {t}
         (argnames : type.for_each_lhs_of_arrow ltype t)
         (args : type.for_each_lhs_of_arrow API.interp_type t)
-        (flat_args : list Semantics.word) s mem :
+        (flat_args : list word) s : forall (mem : mem),
     equivalent_flat_args args flat_args s mem ->
     (exists l,
         map.of_list_zip (flatten_argnames argnames) flat_args = Some l).
@@ -261,7 +262,7 @@ Section Flatten.
 
   Lemma flatten_listonly_samelength {t}
         (names : listonly_base_ltype t) (value : base.interp t) :
-    forall (words : list Semantics.word) s R mem,
+    forall (words : list word) s R mem,
       sep (equivalent_listonly_flat_base value words s) R mem ->
       length words = length (flatten_listonly_base_ltype names).
   Proof.
