src/Bedrock/Group/Point.v
@@ -8,14 +8,20 @@ Section Gallina.
 End Gallina.
 
 Section Compile.
-  Context {semantics : Semantics.parameters}
-          {semantics_ok : Semantics.parameters_ok semantics}.
+  Context {width: Z} {BW: Bitwidth width} {word: word.word width} {mem: map.map word Byte.byte}.
+  Context {locals: map.map String.string word}.
+  Context {env: map.map String.string (list String.string * list String.string * Syntax.cmd)}.
+  Context {ext_spec: bedrock2.Semantics.ExtSpec}.
+  Context {word_ok : word.ok word} {mem_ok : map.ok mem}.
+  Context {locals_ok : map.ok locals}.
+  Context {env_ok : map.ok env}.
+  Context {ext_spec_ok : Semantics.ext_spec.ok ext_spec}.
   Context {field_parameters : FieldParameters}
           {field_representation : FieldRepresentation}.
 
   Lemma compile_point_assign :
-    forall (locals: Semantics.locals) (mem: Semantics.mem)
-           (locals_ok : Semantics.locals -> Prop)
+    forall (l: locals) (mem: mem)
+           (locals_ok : locals -> Prop)
       tr retvars R functions T (pred: T -> _ -> _ -> Prop)
       (x y : F M_pos) k k_impl,
       let v := (x, y) in
@@ -26,14 +32,14 @@ Section Compile.
                                                (fun y => k (x, y)))))
        and-returning retvars
        and-locals-post locals_ok
-       with-locals locals and-memory mem and-trace tr and-rest R
+       with-locals l and-memory mem and-trace tr and-rest R
        and-functions functions) ->
       (let head := v in
        find k_impl
        implementing (pred (dlet head k))
        and-returning retvars
        and-locals-post locals_ok
-       with-locals locals and-memory mem and-trace tr and-rest R
+       with-locals l and-memory mem and-trace tr and-rest R
        and-functions functions).
   Proof.
     repeat straightline'. eauto.
